compute.v
@@ -9,7 +9,7 @@ Module M := FSetAVL.Make(Z_as_OT).
 
 Eval compute in (M.min_elt (M.union'  (M.add 3 (M.add 0 (M.empty))) (M.add 1 (M.add 2 (M.empty))))).
 
-Module MI := FSetAVL_int.Make(Int.Z_as_Int)(Z_as_OT).
+Module MI := FSetAVL_int.Make(Z_as_OT).
 
 Eval compute in (MI.min_elt (MI.union'  (MI.add 3 (MI.add 0 (MI.empty))) (MI.add 1 (MI.add 2 (MI.empty))))).
 
